proofs/fstar/extraction/Golden_dkg.Schnorr_pok.fst
@@ -3,6 +3,8 @@ module Golden_dkg.Schnorr_pok
 open FStar.Mul
 open Core_models
 
+include Golden_dkg.Bundle {compute_challenge as compute_challenge}
+
 include Golden_dkg.Bundle {t_SchnorrPoK as t_SchnorrPoK}
 
 include Golden_dkg.Bundle {impl as impl}
@@ -12,5 +14,3 @@ include Golden_dkg.Bundle {impl_1 as impl_1}
 include Golden_dkg.Bundle {prove as prove}
 
 include Golden_dkg.Bundle {verify as verify}
-
-include Golden_dkg.Bundle {compute_challenge as compute_challenge}
