proofs/fstar/extraction/Golden_dkg.Types.fst
@@ -7,6 +7,8 @@ include Golden_dkg.Bundle {t_SessionId as t_SessionId}
 
 include Golden_dkg.Bundle {SessionId as SessionId}
 
+include Golden_dkg.Bundle {impl_4 as impl_4}
+
 include Golden_dkg.Bundle {impl_5 as impl_5}
 
 include Golden_dkg.Bundle {impl_6 as impl_6}
@@ -16,8 +18,6 @@ include Golden_dkg.Bundle {impl_7 as impl_7}
 include Golden_dkg.Bundle {impl_8 as impl_8}
 
 include Golden_dkg.Bundle {impl_9 as impl_9}
-
-include Golden_dkg.Bundle {impl_10 as impl_10}
 
 include Golden_dkg.Bundle {impl__random as impl_SessionId__random}
 
@@ -30,12 +30,6 @@ include Golden_dkg.Bundle {impl_1__new as impl_SecretScalar__new}
 include Golden_dkg.Bundle {impl_1__inner as impl_SecretScalar__inner}
 
 include Golden_dkg.Bundle {impl_2 as impl_2}
-
-include Golden_dkg.Bundle {impl_3 as impl_3}
-
-include Golden_dkg.Bundle {ark_to_bytes as ark_to_bytes}
-
-include Golden_dkg.Bundle {ark_from_bytes as ark_from_bytes}
 
 include Golden_dkg.Bundle {t_Ciphertext as t_Ciphertext}
 
@@ -69,7 +63,7 @@ include Golden_dkg.Bundle {impl_20 as impl_20}
 
 include Golden_dkg.Bundle {t_Participant as t_Participant}
 
-include Golden_dkg.Bundle {impl_4__new as impl_Participant__new}
+include Golden_dkg.Bundle {impl_3__new as impl_Participant__new}
 
 include Golden_dkg.Bundle {t_DkgConfig as t_DkgConfig}
 
